---
title: 'MTH 463 \n Homework #4'
author: "Duncan Gates"
date: "`r format(Sys.time(), '%d %B, %Y')`"
output: 
  prettydoc::html_pretty:
    theme: leonids # Other options are cayman, tactile, architect, leonids, hpstr
    highlight: vignette
    math: katex #Instead of mathjax so it works offline
documentclass: book
classoption:
  - twocolumn
  - landscape
papersize: a5
linestretch: 1.5
fontsize: 12pt
links-as-notes: true
header-includes:
  - \usepackage{indentfirst}
---

```{r setup, include=FALSE}
knitr::opts_chunk$set(echo = TRUE)
# library(pagedown)
# setwd("/Users/dunk/Classes/MTH463/Homework 4")
# pagedown::chrome_print(input = "Homework-4.html",
#                       output = "Homework4.pdf")
```

## Problem 1

I check that f(x) is a probability density function by finding if the cumulative distribution function is 1 

$$
\begin{aligned}
\int_{-\infty}^{\infty}f(x)dx&=\int_{-2}^{\infty}\frac{8dx}{x^3} \\
&=\Bigg[\frac{8x^{-2}}{-2}\Bigg]_{2}^{\infty} \\
&= \boxed{1}
\end{aligned}
$$
So we know that f(x) is indeed a probability density function.

To find $P(X>5)$

$$
\begin{aligned}
P(X>5)&=\int_{5}^{\infty}\frac{8dx}{x^3} \\
&= \Bigg[\frac{8x^{-2}}{-2}\Bigg]_{5}^{\infty} \\
&= \boxed{\frac{4}{25}}
\end{aligned}
$$

To find $E[X]$ we use 

$$
\begin{aligned}
E[X]&=\int_{-\infty}^{\infty}xf(x)dx \\
&=\int_{2}^{\infty}\frac{8dx}{x^2} \\
&=\Bigg[\frac{8x^{-1}}{-1}\Bigg]_{2}^{\infty} \\
&=\boxed{4}
\end{aligned}
$$


## Problem 2

I find c by integrating knowing the probability density function is equal to 1

$$
\begin{aligned}
1&=\int_{-\infty}^{\infty}f(x)dx \\
&= \int_{1}^{2}c(x-1)^4dx \\
&= \Bigg[\int_{1}^{2}\frac{c(x-1)^5}{5}\Bigg]_1^2 \\
&=\frac{c}{5} \\
\text{therefore, } &\boxed{ c=5}
\end{aligned}
$$

To find $E[X]$ we have 

$$
\begin{aligned}
E[X]&=\int_{-\infty}^{\infty}xf(x)dx \\
&=\int_{1}^{2}5x(x-1)^4dx \\
&=\int_{1}^{2}5((x-1)+1)(x-1)^4dx \\
&=\int_{1}^{2}5(x-1)^5dx+\int_{1}^{2}5(x-1)^4dx \\
&=\Bigg[\frac{5(x-1)^6}{6}\Bigg]_1^2+1 \\
&= \frac{5}{6}+1 \\
&= \boxed{\frac{11}{6}}
\end{aligned}
$$

## Problem 3 

$$
\begin{aligned}
1&= \int_{-\infty}^{\infty}f(x)dx \\
&= \int_0^1(ax^2+bx)dx \\
&= \Bigg[ax^3\frac{1}{3}+bx^2\frac{1}{2}\Bigg] \\
&= \frac{1}{3}a+\frac{1}{2}b
\end{aligned}
$$

$$
\begin{aligned}
0.75&=E(X) \\
&=\int_{-\infty}^{\infty}xf(x)dx \\
&=\int_{0}^{1}(ax^3+bx^2)dx \\
&= \Bigg[a\frac{x^4}{4}+b\frac{x^3}{3}\Bigg]^1_0 \\
&=\frac{1}{4}a+\frac{1}{3}b
\end{aligned}
$$

So we have $1 = \frac{1}{3}a+\frac{1}{2}b$ and $0.75= \frac{1}{4}a+\frac{1}{3}b$ which reduces to $b=0, a = 3$.

Therefore,

$$
\begin{aligned}
E(X^2)&=\int_{-\infty}^{\infty}x^2f(x)dx \\
&=\int_{1}^{0}3x^4dx \\
&= \frac{3x^5}{5}\Bigg|_0^1 \\
&= \boxed{\frac{3}{5}}
\end{aligned}
$$

and,

$$
\begin{aligned}
Var(X)&= E(X^2)-E(X)^2 \\
&= \frac{3}{5} - {0.75}^2 \\
&= \boxed{0.0375}
\end{aligned}
$$

## Problem 4

$$
\begin{aligned}
P(1<X<3)&=\int_1^3F(x)dx \\
&=\int_{-\infty}^3F(x)dx- \int_{-\infty}^1F(x)dx \\
&=F(3)-F(1) \\
&= \frac{15}{6}-\frac{3}{4} \\
&= \boxed{\frac{3}{16}}
\end{aligned}
$$


## Problem 5

Given $4x^2+4xY-Y+6=0$ with $\lambda=3$, the roots of Y ($\frac{-4Y \pm \sqrt{16Y^2+16(Y-6)}}{8}$) will only be positive iff $16Y^2+16(Y-6) \ge 0$. So we need to find 

$$
\begin{aligned}
P(16Y^2+16(Y-6) \ge 0)&=P(Y^2+Y-6 \ge 0) \\
&=P((Y+3)*(Y-2) \ge 0) \\
&=P(Y \le -3) + P(Y \ge 2) \\
&=0+e^{-2\lambda} \\
&= \boxed{e^{-6}}
\end{aligned}
$$


## Problem 6

$$
\begin{aligned}
\tau(\alpha + 1)&=\int_0^{\infty}e^{-y}y^{\alpha}dy \\
&= \int_0^{\infty}(-e^{-y})'y^{\alpha}dy \\
&=(-e^{-y}y^\alpha)\Bigg|_0^{\infty}-\int_0^{\infty}e^{-y}(y^{\alpha})'dy \\
&=0 + \int_0^{\infty}e^{-y}y^{\alpha-1}dy \\
&=\alpha \tau(\alpha) \\
\tau(1)&=\int_0^{\infty}e^{-y}dy \\
&=1=0!
\end{aligned}
$$

Therefore $\tau(2)=1*\tau(1)=1!$

## Problem 7

$$
\begin{aligned}
E[X^k]&=\int_0^{\infty}(\frac{y}{\lambda})^ke^{-y}dy \\
&=\frac{1}{\lambda^k}\int_0^{\infty}e^{-y}y^{(k+1)-1}dy \\
&=\frac{\tau(k+1)}{\lambda^k} \\
&=\frac{k!}{\lambda^k} 
\end{aligned}
$$


## Problem 8

$$
\begin{aligned}
E[e^{-x}]&=\frac{1}{\tau(\alpha)}\int_0^{\infty}\lambda e^{-x}e^{-\lambda x}(\lambda x)^{\alpha -1}dx \\
&=\frac{\lambda}{\tau(\alpha)}\int_0^{\infty}e^{-(\lambda + 1) x}(x)^{\alpha -1}dx && \text{Let } y = (\lambda + 1)x \\
&=\frac{\lambda}{\tau(\alpha)}\int_0^{\infty}e^{-y}\frac{y^{\alpha - 1}}{(\lambda + 1)^{\alpha - 1}}\frac{1}{\lambda + 1}dy \\
&=\Bigg(\frac{\lambda}{\lambda+1}\Bigg)^\alpha\frac{1}{\tau(\alpha)}\int_0^{\infty}e^{-y}y^{\alpha-1}dy \\
&=\Bigg(\frac{\lambda}{\lambda+1}\Bigg)^\alpha
\end{aligned}
$$


## Problem 9

We have $t>0$, $f(t)=\lambda e^{-\lambda t}$, $F(t)=1-e^{-\lambda t}$.

$$
\begin{aligned}
h(t)&=\frac{f(t)}{1-F(t)} \\
&=\frac{\lambda e^{-\lambda t}}{1-(1-e^{-\lambda t})} \\
&= \lambda
\end{aligned}
$$

The memorylessness property therefore makes it such that the "hazard rate" is constant at all times







